src/SDK/Deserialize.dfy
@@ -2,7 +2,7 @@
 // SPDX-License-Identifier: Apache-2.0
 
 include "MessageHeader.dfy"
-include "Materials.dfy"
+include "../AwsCryptographicMaterialProviders/Materials.dfy"
 include "EncryptionContext.dfy"
 include "AlgorithmSuite.dfy"
 
@@ -35,7 +35,7 @@ module Deserialize {
   import opened Wrappers
   import opened UInt = StandardLibrary.UInt
   import UTF8
-  import Materials
+  import MaterialProviders.Materials
   import EncryptionContext
 
 
